Defs2.thy
@@ -1,0 +1,79 @@
+theory Defs2
+  imports Lemmas
+begin
+
+nominal_function ctor_data_app_subst :: "\<tau> \<Rightarrow> bool" where
+  "ctor_data_app_subst (TyVar _) = False"
+| "ctor_data_app_subst (TyData _) = True"
+| "ctor_data_app_subst TyArrow = False"
+| "ctor_data_app_subst (TyApp \<tau>1 _) = ctor_data_app_subst \<tau>1"
+| "ctor_data_app_subst (TyForall _ _ _) = False"
+proof goal_cases
+  case (3 P x)
+  then show ?case by (cases x rule: \<tau>.exhaust) auto
+qed (auto simp: eqvt_def ctor_data_app_subst_graph_aux_def)
+nominal_termination (eqvt) by lexicographic_order
+
+nominal_function ctor_args :: "\<tau> \<Rightarrow> \<tau> list option" where
+  "ctor_args (TyVar _) = None"
+| "ctor_args (TyData T) = Some []"
+| "ctor_args TyArrow = None"
+| "ctor_args (TyApp (TyApp TyArrow \<tau>1) \<tau>2) = (case ctor_args \<tau>2 of
+    Some tys \<Rightarrow> Some (\<tau>1#tys)
+  | None \<Rightarrow> None)"
+| "ctor_args (TyApp (TyApp (TyVar a) \<tau>1) \<tau>2) = (if ctor_data_app_subst (TyApp (TyApp (TyVar a) \<tau>1) \<tau>2) then Some [] else None)"
+| "ctor_args (TyApp (TyApp (TyData T) \<tau>1) \<tau>2) = (if ctor_data_app_subst (TyApp (TyApp (TyData T) \<tau>1) \<tau>2) then Some [] else None)"
+| "ctor_args (TyApp (TyApp (TyApp \<tau>1' \<tau>2') \<tau>1) \<tau>2) = (if ctor_data_app_subst (TyApp (TyApp (TyApp \<tau>1' \<tau>2') \<tau>1) \<tau>2) then Some [] else None)"
+| "ctor_args (TyApp (TyApp (TyForall a k e) \<tau>1) \<tau>2) = (if ctor_data_app_subst (TyApp (TyApp (TyForall a k e) \<tau>1) \<tau>2) then Some [] else None)"
+| "ctor_args (TyApp (TyVar a) \<tau>2) = (if ctor_data_app_subst (TyApp (TyVar a) \<tau>2) then Some [] else None)"
+| "ctor_args (TyApp (TyData T) \<tau>2) = (if ctor_data_app_subst (TyApp (TyData T) \<tau>2) then Some [] else None)"
+| "ctor_args (TyApp TyArrow \<tau>2) = (if ctor_data_app_subst (TyApp TyArrow \<tau>2) then Some [] else None)"
+| "ctor_args (TyApp (TyForall a k e) \<tau>2) = (if ctor_data_app_subst (TyApp (TyForall a k e) \<tau>2) then Some [] else None)"
+| "ctor_args (TyForall _ _ _) = None"
+proof goal_cases
+  case 1
+  then show ?case by (auto simp: eqvt_def ctor_args_graph_aux_def split!: option.splits)
+next
+  case (3 P x)
+  then show ?case
+  proof (cases x rule: \<tau>.exhaust)
+    case outer: (TyApp \<tau>1 \<tau>2)
+    then show ?thesis using 3
+    proof (cases \<tau>1 rule: \<tau>.exhaust)
+      case (TyApp \<sigma>1 \<sigma>2)
+      then show ?thesis using outer 3 by (cases \<sigma>1 rule: \<tau>.exhaust) auto
+    qed auto
+  qed auto
+qed auto
+nominal_termination (eqvt) by lexicographic_order
+
+nominal_function subst_ctor :: "\<tau> \<Rightarrow> \<tau> list \<Rightarrow> \<tau> list option" where
+  "subst_ctor (TyVar _) _ = None"
+| "subst_ctor TyArrow _ = None"
+| "subst_ctor (TyData _) [] = Some []"
+| "subst_ctor (TyData _) (_#_) = None"
+| "subst_ctor (TyApp \<tau>1 \<tau>2) [] = ctor_args (TyApp \<tau>1 \<tau>2)"
+| "subst_ctor (TyApp _ _) (_#_) = None"
+| "subst_ctor (TyForall _ _ _) [] = None"
+| "subst_ctor (TyForall a _ e) (\<tau>#\<tau>s) = subst_ctor e[\<tau>/a] \<tau>s"
+proof goal_cases
+  case (3 P x)
+  then obtain t xs where P: "x = (t, xs)" by fastforce
+  then show ?case using 3
+  proof (cases t rule: \<tau>.exhaust)
+    case TyData
+    then show ?thesis using P 3 by (cases xs) auto
+  next
+    case TyApp
+    then show ?thesis using P 3 by (cases xs) auto
+  next
+    case TyForall
+    then show ?thesis using P 3 by (cases xs) auto
+  qed auto
+next
+  case (39 a k e \<tau> \<tau>s a' k' e' \<tau>' \<tau>s')
+  then show ?case by (metis Pair_inject \<tau>.eq_iff(5) list.inject subst_same(2))
+qed (auto simp: eqvt_def subst_ctor_graph_aux_def)
+nominal_termination (eqvt) by lexicographic_order
+
+end
