Nominal2_Lemmas.thy
@@ -102,4 +102,9 @@ lemma Projr_permute: "\<exists>y. f = Inr y \<Longrightarrow> p \<bullet> projr 
 lemma pair3_eqvt[simp]: "(a \<leftrightarrow> b) \<bullet> (x, y, z) = ((a \<leftrightarrow> b) \<bullet> x, (a \<leftrightarrow> b) \<bullet> y, (a \<leftrightarrow> b) \<bullet> z)"
   by (simp split: prod.splits)
 
+lemma eqvt_fBall[eqvt]: "p \<bullet> fBall s f = fBall (p \<bullet> s) (p \<bullet> f)"
+  apply auto
+  apply (metis eqvt_bound eqvt_lambda fBallE in_fset_eqvt permute_pure)
+  by (metis eqvt_apply fBallE fBallI in_fset_eqvt permute_pure)
+
 end
